rt abstract: updates for timeout exceptions (SELFOUR-277)

spec/abstract/Invocations_A.thy
@@ -50,6 +50,7 @@ datatype tcb_invocation =
   | CopyRegisters machine_word machine_word bool bool bool bool arch_copy_register_sets
   | ThreadControl machine_word cslot_ptr
                   (tc_new_fault_handler: "(cap * cslot_ptr) option")
+                  (tc_new_timeout_handler: "(cap * cslot_ptr) option")
                   (tc_new_mcpriority: "word8 option")
                   (tc_new_priority: "word8 option")
                   (tc_new_croot: "(cap * cslot_ptr) option")
@@ -61,12 +62,13 @@ datatype tcb_invocation =
   | NotificationControl "obj_ref" "obj_ref option"
 
 datatype sched_context_invocation =
-    InvokeSchedContextBind obj_ref cap
+    InvokeSchedContextConsumed obj_ref "data list"
+  | InvokeSchedContextBind obj_ref cap
   | InvokeSchedContextUnbindObject obj_ref cap
   | InvokeSchedContextUnbind obj_ref
 
 datatype sched_control_invocation =
-    InvokeSchedControlConfigure obj_ref ticks ticks nat
+    InvokeSchedControlConfigure obj_ref ticks ticks nat badge
 
 datatype irq_control_invocation =
     IRQControl irq cslot_ptr cslot_ptr
